# LexicalAnalyzer-Haskell
Grammar:
G = (V, , P, E )
V = { E, A, 0, 1, x, y, +, -, *, (, ) },
 = { x, y, +, -, *, /, (, ) }
P: – E 0 | 1 | x | y | (EAE) – A + | - | * | /
Entry Details
The input expression must be placed in the main function of the code and
your modification must be done manually.
4. Output Details
If the input expression is a word generated by the grammar of
aritimeticas expressions being used to call the main
return true, if not, return false. Examples:
(0 + 1) = True
(0 + 1x) + x = False
